---
title: "CT Convolution"
---

## Review CT LTI systems and superposition property

Recall the superposition property of LTI systems. If a CT system is LTI
then the superposition property holds. Given a system where
$$x_i(t) \mapsto y_i(t) \; \forall\; i$$ then
$$\sum\limits_{i} a_i x_i(t) \mapsto \sum\limits_{i} a_i y_i(t)$$

Superposition enables a powerful problem reduction strategy. The overall
idea for is that if:

- we can write an arbitrary signal as a sum of simple signals, and

- we can determine the response to the simple signals, then

- we can easily express the output due to the input using superposition

This will be a recurring pattern in this course. In this lecture, the
simple signals are weighted, time shifts of one signal, the delta
function, $\delta(t)$.

## Convolution Integral

To derive this we start with the sifting property of the CT impulse
function (from chapter 2)
$$\int\limits_{a}^{b} x(t)\delta(t-t_0) \; dt = x(t_0)$$ for any
$a < t_0 < b$. A slight change of variables ($t_0 \rightarrow \tau$) and
limits ($a \rightarrow -\infty$ and $b \rightarrow \infty$) gives:
$$x(t) = \int\limits_{-\infty}^{\infty} x(\tau)\delta(t-\tau) \; d\tau$$
showing that we can write any CT signal as an infinite sum (integral) of
weighted and time-shifted impluse functions.

Let $h(t)$ be the CT *impulse response*, the output due to the input
$\delta(t)$, i.e. $\delta(t) \mapsto h(t)$. Then if the system is
time-invariant: $\delta(t-\tau) \mapsto h(t-\tau)$ and by superposition
if the input is writen as
$$x(t) = \int\limits_{-\infty}^{\infty} x(\tau)\delta(t-\tau) \; d\tau$$
then the output is given by
$$y(t) = \int\limits_{-\infty}^{\infty} x(\tau)h(t-\tau) \; d\tau = x(t) * h(t)$$
This is called the *convolution integral* .

It is worth pausing here to see the signifigance. For a LTI CT system,
if I know its impulse response $h(t)$, I can find the response due to
**any** input using convolution. For this reason the impulse response is
another way to represent an LTI system.

## Graphical View of the Convolution Integral.

Let us break the convolution expression down into pieces. In its general
form the convolution of two signals $x_1(t)$ and $x_2(t)$ is
$$x_1(t) * x_2(t) = \int\limits_{-\infty}^{\infty} x_1(\tau)x_2(t-\tau) \; d\tau$$

Suppose $x_1(t)$ and $x_2(t)$ are signals that look like

![The two signals being convolved.](images/convolution-explain1){fig-align="center" fig-alt="diagram showing the signals being used for convolution"}

Then $x_1(\tau)$ and $x_2(-\tau)$ look like

![The second signal reflected.](images/convolution-explain2){fig-align="center" fig-alt="diagram showing the signals being used for convolution, see caption"}


The signal $x_2(t-\tau)$ is $x_2(-\tau)$ shifted by $t$ (since
$x_2(-\tau+t)= x_2(t-\tau)$) and then looks like


![The second reflected signal, shifted.](images/convolution-explain3){fig-align="center" fig-alt="diagram showing the signals being used for convolution, see caption"}


Then the integrand of convolution is the product $x_1(\tau)x_2(t-\tau)$
whose plot depends of the value of $t$. Some examples, where the
individual signals are dashed and their product is in bold:


![The product of the two signals under the convolution integrand.](images/convolution-explain4){fig-align="center" fig-alt="diagram showing the signals being used for convolution, see caption"}


Then convolution is the total integral of the product (bold curves
above) for that value of $t$. For the example above we see the integral
will be zero for $t$ less than $t_0$ since the two signals do not
overlap and their product is zero. For $t_0 < t < t_1$ the signals
overap and the product is non-zero, and the effective bounds of
integration are $[t_0,t]$. For $t > t_1$ the signals again overap and
the product is non-zero, but the effective bounds of integration are
$[t_0,t_1]$.

## Examples of CT Convolution

:::{.example}
::::{.example-header}
Example
::::
::::{.example-container}

Consider the convolution of two unit step functions.
$$u(t) * u(t) = \int\limits_{-\infty}^{\infty} u(\tau)u(t-\tau) \; d\tau$$
The product $u(\tau) u(t-\tau)$ is non-zero only when $t\geq 0$ as
illustrated here


![The product of the two step signals under the convolution integrand.](images/convolution-step){fig-align="center" fig-alt="diagram showing the signals being used for convolution, see caption"}


The convolution integral is then the shaded area
$$u(t) * u(t) = \left\{ \begin{array}{lc}
  0 & t< 0\\
  \int\limits_{0}^{t} d\tau = t  & t \geq 0\\
\end{array}\right.$$ Combining this back into a single expression gives:
$$u(t) * u(t) = tu(t)$$ Thus the convolution of two step signals is a
ramp signal.

::::
:::

:::{.example}
::::{.example-header}
Example
::::
::::{.example-container}

Let $x_1(t) = u(t)$ and $x_2(t) = e^{-at}u(t)$ for constant
$a\in\mathbb{C}$, then
$$u(t) * e^{-at}u(t) = \int\limits_{-\infty}^{\infty} u(\tau)e^{-a(t-\tau)}u(t-\tau) \; d\tau$$
Similar to the previous example, the product
$u(\tau) e^{-a(t-\tau)} u(t-\tau)$ is non-zero only when $t\geq 0$


![The product of the two step signals under the convolution integrand.](images/convolution-expstep){fig-align="center" fig-alt="diagram showing the signals being used for convolution, see caption"}


The convolution integral is then the shaded area
$$u(t) * e^{-at}u(t) = \left\{ \begin{array}{lc}
  0 & t< 0\\
  \int\limits_{0}^{t} e^{-a(t-\tau)} d\tau = \frac{1-e^{-at}}{a}  & t \geq 0\\
\end{array}\right.$$ Combining this back into a single expression gives:
$$u(t) * e^{-at}u(t) = \frac{1-e^{-at}}{a}u(t)$$ 

::::
:::

:::{.example}
::::{.example-header}
Example
::::
::::{.example-container}

Let $x_1(t) = \delta(t)$ and $x_2(t)$ be an arbitrary signal. Then
$$\delta(t) * x_2(t) = \int\limits_{-\infty}^{\infty} \delta(\tau)x_2(t-\tau) \; d\tau$$
By the sifting property of the delta function this evaluates to
$$\delta(t) * x_2(t) = x_2(t)$$ or in other words convolution with a
delta function just results in the signal it was convolved with. That is
it acts like the identity function, with respect to convolution.

::::
:::


The appendix lists several CT convolution results.

## Properties of CT Convolution

There are several useful properties of convolution. We do not prove
these here, but it is not terribly difficult to do so. Given signals
$x_1(t)$, $x_2(t)$, and $x_3(t)$:

Communative Property

:   The ordering of the signals does not matter.
    $$x_1(t) * x_2(t) = x_2(t) * x_1(t)$$

Distributive Property

:   Convolution is distributed over addition.
    $$x_1(t) * \left[x_2(t) + x_3(t)\right] = \left[x_1(t) * x_2(t) \right] + \left[x_1(t) * x_3(t) \right]$$

Associative Property

:   The order of convolution does not matter.
    $$x_1(t) * \left[x_2(t) * x_3(t)\right] = \left[x_1(t) * x_2(t) \right] * x_3(t)$$

Time Shift

:   Given $x_3(t) = x_1(t) * x_2(t)$ then for time shifts
    $\tau_1, \tau_2 \in \mathbb{R}$
    $$x_1(t-\tau_1) * x_2(t-\tau_2) = x_3(t-\tau_1 - \tau_2)$$

Multiplicative Scaling

:   Given $x_3(t) = x_1(t) * x_2(t)$ then for constants
    $a,b \in \mathbb{C}$
    $$\left[a\, x_1(t)\right] * \left[b\, x_2(t)\right] = a\, b\, x_3(t)$$

These properties can be used in combination with a table like that above
to compute the convolution of a wide variety of signals without
evaluating the integrals.

:::{.example}
::::{.example-header}
Example
::::
::::{.example-container}

Here is a simple example. Let $x_1(t) = e^tu(t)$ and
$x_2(t) = 2\delta(t) + 5e^{-3t}u(t)$.
$$x_1(t) * x_2(t) =  e^tu(t) * \left[2\delta(t) + 5e^{-3t}u(t)\right]$$
Using the distributive property
$$x_1(t) * x_2(t) =  2\left[\delta(t) * e^tu(t)\right]  + 5\left[e^tu(t) * e^{-3t}u(t)\right]$$
Using previously derived results involving the delta function and the
table row 3
$$x_1(t) * x_2(t) = 2 e^t\, u(t) + 5\left[ \frac{e^t-e^{-3t}}{4}\right]u(t)$$
Doing some simplification gives the result
$$x_1(t) * x_2(t) = \left[ \frac{13}{4}e^t-\frac{5}{4}e^{-3t}\right]u(t)$$

::::
:::


:::{.example}
::::{.example-header}
Example
::::
::::{.example-container}

Here is a more complicated example. Let $x_1(t) = 2e^{-5t}u(t-1)$ and
$x_2(t) = \left(1-e^{-t}\right)u(t)$.
$$x_1(t) * x_2(t) = \left[2e^{-5t}u(t-1)\right] * \left[\left(1-e^{-t}\right)u(t)\right]$$
We first rewrite
$e^{-5t}u(t-1)=e^{-5}e^{-5(t-1)}u(t-1) = e^{-5}e^{-5t}u(t)\Big|_{t=t-1}$
so that we can remove the time shift
$$x_1(t) * x_2(t) = 2e^{-5}\left[e^{-5t}u(t)\right] * \left[\left(1-e^{-t}\right)u(t)\right]\Big|_{t=t-1}$$
We now apply the distributive property
$$x_1(t) * x_2(t) = 2e^{-5}\left[\left(e^{-5t}u(t) * u(t)\right) - \left(e^{-5t}u(t)* e^{-t}u(t)\right)\right]\Big|_{t=t-1}$$
Using the table rows 1 and 3 we get
$$x_1(t) * x_2(t) = 2e^{-5}\left[\frac{1}{5}\left(1-e^{-5t}\right)u(t) + \frac{1}{4}\left(e^{-5t} - e^{-t}\right)u(t)\right]\Big|_{t=t-1}$$
Combining terms we simplify to
$$x_1(t) * x_2(t) = 2e^{-5}\left[\frac{1}{5} - \frac{1}{4}e^{-t} + \frac{1}{20}e^{-5t} \right]u(t)\Big|_{t=t-1}$$
Replacing the time shift gives the final result
$$x_1(t) * x_2(t) = 2e^{-5}\left[\frac{1}{5} - \frac{1}{4}e^{-(t-1)} + \frac{1}{20}e^{-5(t-1)} \right]u(t-1)$$
which can be cleaned up a bit more by distributing the leading term
$$x_1(t) * x_2(t) =\left[\frac{2}{5}e^{-5} -\frac{1}{2}e^{-(t+4)} +\frac{1}{10}e^{-5t}\right]u(t-1)$$

::::
:::


