---
title: "DT Fourier Transform"
---

Recall the complex exponential $z^{n}$ for $z\in\mathbb{C}$ is the
Eigenfunction of DT LTI systems. If we can decompose an input into a
(possibly infinite) sum of such signals, we can easily determine the
output using the superposition principle. In this section we consider
the decomposition when the input is aperiodic, called the DT *Fourier
Transform* (DTFT).

In contrast to the DT Fourier series, in this case the complex exponent
of the Eigenfunction becomes $z = e^{j\omega}$ a continuous variable,
and the decomposition is an uncountably infinite sum (integral). This
gives the input-output relationship for a stable DT LTI system as
$$x[n] = \frac{1}{2\pi}\int\limits_{2\pi} X\left(e^{j\omega}\right) \, e^{j \omega n}\; d\omega \;\longrightarrow\; y[n] = \frac{1}{2\pi}\int\limits_{2\pi} H\left(e^{j\omega}\right) X\left(e^{j\omega}\right) \, e^{j \omega n}\; d\omega$$
where $H\left(e^{j \omega}\right)$ are the Eigenvalues, again called the
*frequency response*. We now turn to determining under what
circumstances the decomposition exists and how to find the function
$X\left(e^{j\omega}\right)$.

**Note:** The notation $X\left(e^{j\omega}\right)$ can be confusing. It
just emphasizes that $z \rightarrow e^{j\omega}$. The expressions are
functions of the independent variable $\omega$.

## Analysis and Synthesis Equations

Consider the Fourier series of $x[n]$, a periodically extended
finite-length DT signal $\tilde{x}[n]$, e.g.

![Example of a finite-length DT signal and its periodic extension.](figures/fig17_1){fig-align="center" fig-alt="See the caption."}

where $\tilde{x}[n]$ is zero outside the range $[N_1,N_2]$. Since
$x[n] = \tilde{x}[n]$ over the interval $-N_1$ to $N_2$
$$a_k = \frac{1}{N}\sum\limits_{n = -N_1}^{N_2} \tilde{x}[n] e^{-j\frac{2\pi}{N}kn} = \frac{1}{N}\sum\limits_{n = -\infty}^{\infty} x[n] e^{-j\frac{2\pi}{N}kn}$$
Define the function
$X\left(e^{j\omega}\right) = \sum\limits_{n = -\infty}^{\infty} x[n] e^{-j\omega n}$,
then $$a_k = \frac{1}{N} X\left(e^{jk\omega_0}\right)$$ are samples of
$X\left(e^{j\omega}\right)$ at locations that are multiples of
$\omega_0 = \frac{2\pi}{N}$. Substituting back into the synthesis
equation
$$\tilde{x}[n] = \sum\limits_{k = -N_1}^{N_2} a_k e^{j\frac{2\pi}{N}kn} = \sum\limits_{k = -N_1}^{N_2} \frac{1}{N} X\left(e^{jk\omega_0}\right) e^{jk\omega_0 n}$$
Now note that $N = \frac{2\pi}{\omega_0}$ so that
$$\tilde{x}[n] = \frac{1}{2\pi} \sum\limits_{k = -N_1}^{N_2} X\left(e^{jk\omega_0}\right) e^{jk\omega_0 n} \; \omega_0$$
Now let $N \rightarrow \infty$.

\begin{aligned}
  \lim_{N\rightarrow \infty} \tilde{x}[n] &= \lim_{N\rightarrow \infty} \frac{1}{2\pi} \sum\limits_{k = -N_1}^{N_2} X\left(e^{jk\omega_0}\right) e^{jk\omega_0 n} \; \omega_0\\
  x[n] &= \frac{1}{2\pi} \int_{2\pi} X\left(e^{j\omega}\right) e^{j\omega n} \; d\omega
\end{aligned}

This is shown graphically in the figure below. As $N$
approaches infinity the sampling of the unit circle becomes infinite,
and the summation approaches an integral.

![Illustration of the limit process leading the the inverse DT Fourier Transform.](figures/fig17_2){fig-align="center" fig-alt="See the caption."}

This gives the *DT Fourier Transform Pair*. The Analysis Equation or
Forward Transform is:
$$X\left(e^{j\omega}\right) = \sum\limits_{n = -\infty}^{\infty} x[n] e^{-j\omega n}$$
Note $X\left(e^{j\omega}\right)$ must be a periodic function with period
$2\pi$. The Synthesis Equation or Inverse Transform is:
$$x[n] = \frac{1}{2\pi} \int_{2\pi} X\left(e^{j\omega}\right) e^{j\omega n} \; d\omega$$
where the integral is over any $2\pi$ period of $X$.

:::{.example}
::::{.example-header}
Example
::::
::::{.example-container}
Let $x[n] = \delta[n]$

\begin{aligned}
    X\left(e^{j\omega}\right) &= \sum\limits_{n = -\infty}^{\infty} x[n] e^{-j\omega n}\\
    &= \sum\limits_{n = -\infty}^{\infty} \delta[n] e^{-j\omega n}\\
    &= e^{-j\omega (0)}\\
    &= 1
  
\end{aligned}
::::
:::

:::{.example}
::::{.example-header}
Example
::::
::::{.example-container}

Let $x[n] = \left( \gamma \right)^n\; u[n]$

\begin{aligned}
    X\left(e^{j\omega}\right) &= \sum\limits_{n = -\infty}^{\infty} x[n] e^{-j\omega n}\\
    &= \sum\limits_{n = 0}^{\infty} \left( \gamma \right)^n \; e^{-j\omega n}\\
    &= \sum\limits_{n = 0}^{\infty} \left( \gamma e^{-j\omega} \right)^n
  
\end{aligned}

Using the geometric series
$\sum\limits_{n = 0}^{\infty} z^n = \frac{1}{1-z}$ for $|z| < 1$ gives:
$$X\left(e^{j\omega}\right) = \sum\limits_{n = 0}^{\infty} \left( \gamma e^{-j\omega} \right)^n = \frac{1}{1-\gamma e^{-j\omega}} = \frac{e^{j\omega}}{e^{j\omega} - \gamma}$$
If $\mid\gamma e^{-j\omega}\mid < 1$ or equivalently
$\mid \gamma \mid < 1$.

$$\left( \gamma \right)^n\; u[n] \; \stackrel{\mathcal{F}}{\longrightarrow} \; \frac{1}{1-\gamma e^{-j\omega}}$$
Below is a plot of the original signal and the magnitude and phase
spectrum when $\gamma = \tfrac{1}{2}$.

```{python}
#| label: fig-17-example1
#| fig-cap: "Magnitude and phase spectrum for the example."
#| fig-alt: "See Caption."
#| warning: false
#| echo: false

import numpy as np
import matplotlib.pyplot as plt

gamma = 0.5
n = np.arange(-6, 7)
x = np.where(n >= 0, gamma**n, 0)

w = np.arange(-10, 10, step=0.001)
X = 1/(1-gamma*np.exp(-1j*w))

plt.subplot(3,1,1)
plt.stem(n, x)
plt.gca().set_aspect(2)
plt.xticks(n)
plt.xlim(-6,6)
plt.xlabel('n')
plt.ylabel('$x[n]$')
plt.title('Plot of the signal in the example.')

plt.subplot(3,1,2)
plt.plot(w, np.abs(X))
plt.grid()
plt.xlim(-10,10)
plt.xlabel('$\omega$')
plt.ylabel('$|X(e^{j\omega})|$')
plt.title('Magnitude spectrum for the example.')

plt.subplot(3,1,3)
plt.plot(w, np.angle(X))
plt.grid()
plt.xlim(-10,10)
plt.xlabel('$\omega$')
plt.ylabel('$ Angle X(e^{j\omega}) (rad)$')
plt.title('Phase spectrum for the example.')

plt.tight_layout()
plt.show()
```

::::
:::

:::{.example}
::::{.example-header}
Example
::::
::::{.example-container}

Let $$X\left(e^{j\omega}\right) = \left\{ \begin{array}{lc}
    1 & |\omega -2\pi k| < \omega_c\\
    0 & \text{else}
  \end{array}
  \right.
  \; \text{for}\; k\in\mathbb{Z} \;\text{and}\; \omega_c < \pi$$

\begin{aligned}
    x[n] &= \frac{1}{2\pi} \int_{2\pi} X\left(e^{j\omega}\right) e^{j\omega n} \; d\omega\\
    &= \frac{1}{2\pi} \int\limits_{-\omega_c}^{\omega_c}  e^{j\omega n} \; d\omega\\
    &= \frac{1}{2\pi} \frac{1}{jn} e^{j\omega n} \Bigg|_{-\omega_c}^{\omega_c}\\
    &= \frac{1}{\pi n} \left( \frac{1}{2j} e^{j\omega_c n} - \frac{1}{2j} e^{-j\omega_c n} \right)\\
    &= \frac{1}{\pi n} \sin(\omega_c n) = \frac{\omega_c}{\pi}\text{sinc}(\omega_c n)
  
\end{aligned}

::::
:::

:::{.example}
::::{.example-header}
Example
::::
::::{.example-container}

Let
$$X\left(e^{j\omega}\right) = \sum\limits_{k = -\infty}^{\infty} \delta(\omega-\omega_0 -2\pi k)$$
for $-\pi < \omega_0 < \pi$

![Plot of the impulse train in the DT Fourier domain.](figures/fig17_3){fig-align="center" fig-alt="See the caption."}

\begin{aligned}
    x[n] &= \frac{1}{2\pi} \int_{2\pi} X\left(e^{j\omega}\right) e^{j\omega n} \; d\omega\\
    &= \frac{1}{2\pi} \int\limits_{-\pi}^{\pi} \delta(\omega-\omega_0)e^{j\omega n} \; d\omega\\
    &= \frac{1}{2\pi} e^{j\omega_0 n}
  
\end{aligned}

::::
:::

Table [\[table:dtft\]](#table:dtft){reference-type="ref"
reference="table:dtft"} lists several DT Fourier Transform results.

## Existence of the DT Fourier Transform

The example of the exponential $x[n] = \left(\gamma\right)^n\,u[n]$
above showed that for the DT Fourier transform to exist, the Fourier
(analysis) sum must exist. Similar to the CT Fourier transform, a mild
conditions is a sufficient prerequisite for the Fourier transform of a
signal $x[n]$ to exist: it must be absolutely summable
$$\sum\limits_{n = -\infty}^{\infty} |x[n]| < \infty$$

This conditions is not necessary however, and we can extend the Fourier
transform to a broader class of signals, if we allow delta functions in
the transform, as in the sinusoidal examples above.

## Properties of the DT Fourier Transform

There are several useful properties of the DT Fourier Transform that,
when combined with a table of transforms (see Table 5.2, page 392 of
OW), allow us to take the Fourier transform of wide array of signals,
and one, the convolution property, that allows us to determine the
output of a system in the frequency domain easily. We state these here
without proof in rough order of usefulness. See the course text for
detailed derivations.

We use the following notation
$$\mathcal{F}\left\{ x[n] \right\} = X\left(e^{j\omega}\right) = \sum\limits_{n = -\infty}^{\infty} x[n] e^{-j\omega n}$$
$$\mathcal{F}^{-1}\left\{ X\left(e^{j\omega}\right) \right\} = x[n] =  \frac{1}{2\pi} \int_{2\pi} X\left(e^{j\omega}\right) e^{j\omega n} \; d\omega$$
$$x[n] \; \stackrel{\mathcal{F}}{\longleftrightarrow} \;  X\left(e^{j\omega}\right)$$
Important: $X\left(e^{j\omega}\right)$ is periodic in $2\pi$ such that
$$X\left(e^{j(\omega + 2\pi k)}\right) =  X\left(e^{j\omega}\right) \;\text{for}\; k \in \mathbb{Z}$$

- Linearity Property. Let
  $x_1[n] \; \stackrel{\mathcal{F}}{\longleftrightarrow} \; X_1\left(e^{j\omega}\right)$
  and
  $x_2[n] \; \stackrel{\mathcal{F}}{\longleftrightarrow} \; X_2\left(e^{j\omega}\right)$
  then for $a,b\in\mathbb{C}$
  $$a x_1[n] + b x_2[n] \; \stackrel{\mathcal{F}}{\longleftrightarrow} \; a X_1\left(e^{j\omega}\right) + b X_2\left(e^{j\omega}\right)$$
  Example:
  \begin{aligned}
  \mathcal{F}\left\{ 2\left( \frac{1}{2}\right)^nu[n] -5 \left( -\frac{1}{4}\right)^nu[n] \right\} &= \frac{2}{1-\frac{1}{2}e^{-j\omega}} - \frac{5}{1+\frac{1}{4}e^{-j\omega}} 
  \end{aligned}

- Time-shift Property. Let
  $$x[n] \; \stackrel{\mathcal{F}}{\longleftrightarrow} \; X\left(e^{j\omega}\right)$$
  then
  $$x[n-n_0] \; \stackrel{\mathcal{F}}{\longleftrightarrow} \; e^{-j\omega n_0} X\left(e^{j\omega}\right)$$
  Example: $$\mathcal{F}\left\{ \delta[n-5] \right\} = e^{-j5\omega}$$

- Frequency Shift Property. Let
  $$x[n] \; \stackrel{\mathcal{F}}{\longleftrightarrow} \; X\left(e^{j\omega}\right)$$
  then
  $$e^{j\omega_0 n} x[n] \; \stackrel{\mathcal{F}}{\longleftrightarrow} \; X\left(e^{j(\omega-\omega_0)}\right)$$
  Example:
  $$\mathcal{F}^{-1}\left\{ \frac{1}{1-\frac{1}{2}e^{-j\omega}e^{j\frac{\pi}{20}}} \right\} = e^{j\frac{\pi}{20} n} \left( \frac{1}{2}\right)^n u[n]$$

- Conjugation Property. Let
  $$x[n] \; \stackrel{\mathcal{F}}{\longleftrightarrow} \; X\left(e^{j\omega}\right)$$
  then
  $$x^*[n] \; \stackrel{\mathcal{F}}{\longleftrightarrow} \; X^{*}\left(e^{-j\omega}\right)$$
  Thus, if $x[n]$ is real $X\left(e^{j\omega}\right)$ has conjugate
  symmetry $$X\left(e^{-j\omega}\right) = X^*\left(e^{j\omega}\right)$$
  and the magnitude spectrum is an even function and the phase spectrum
  is an odd function.

- Differencing and Accumulation Property. Let
  $$x[n] \; \stackrel{\mathcal{F}}{\longleftrightarrow} \; X\left(e^{j\omega}\right)$$
  then
  $$x[n] - x[n-1] \; \stackrel{\mathcal{F}}{\longleftrightarrow} \; X\left(e^{j\omega}\right) - e^{-j\omega} X\left(e^{j\omega}\right) = \left(1-e^{-j\omega}\right)X\left(e^{j\omega}\right)$$
  and
  $$\sum\limits_{m = -\infty}^{n} x[m] \; \stackrel{\mathcal{F}}{\longleftrightarrow} \; \frac{1}{1-e^{-j\omega}}X\left(e^{j\omega}\right) + \pi X\left(e^{j0}\right)\sum\limits_{k = -\infty}^{\infty} \delta(\omega - 2\pi k)$$

- Time Expansion Property. Let
  $$x[n] \; \stackrel{\mathcal{F}}{\longleftrightarrow} \; X\left(e^{j\omega}\right)$$
  then
  $$x_{(k)}[n] \; \stackrel{\mathcal{F}}{\longleftrightarrow} \; X\left(e^{jk\omega}\right)$$
  where $$x_{(k)}[n] = \left\{ \begin{array}{lc}
      x[n/k] & \text{if}\; n = \; \text{multiple of}\; k\\
      0 & \text{if}\; n \neq \; \text{multiple of}\; k\\ 
    \end{array}
  \right.$$

![Illustration of expansion of a DT signal by a factor of two via insertion of zeros.](figures/fig17_4){fig-align="center" fig-alt="See the caption."}

- Frequency Differentiation Property Let
  $$x[n] \; \stackrel{\mathcal{F}}{\longleftrightarrow} \; X\left(e^{j\omega}\right)$$
  then
  $$n\, x[n] \; \stackrel{\mathcal{F}}{\longleftrightarrow} \; j \frac{d}{d\omega} X\left(e^{j\omega}\right)$$
  Example:
  \begin{aligned}
      \mathcal{F}\left\{ n\left( \frac{1}{8}\right)^n u[n] \right\} &= j \frac{d}{d\omega} \left\{\frac{1}{1-\frac{1}{8}e^{-j\omega}} \right\}\\
      &= j \frac{-\left(-\frac{1}{8} (-j)e^{-j\omega}\right)}{\left( 1-\frac{1}{8}e^{-j\omega} \right)^2}\\
      &= \frac{\frac{1}{8}e^{-j\omega}}{\left( 1-\frac{1}{8}e^{-j\omega} \right)^2}
    
  \end{aligned}

- Parseval's Relation. Let
  $$x[n] \; \stackrel{\mathcal{F}}{\longleftrightarrow} \; X\left(e^{j\omega}\right)$$
  then
  $$\sum\limits_{n = -\infty}^{\infty} |x[n]|^2 \; \stackrel{\mathcal{F}}{\longleftrightarrow} \;
    \frac{1}{2\pi} \int_{2\pi} \left| X\left(e^{j\omega}\right) \right|^2 \; d\omega$$
  The energy is also the integral over one period of the DTFT magnitude
  squared.

- Convolution Property. Recall for a DT LTI system with impulse response
  $h[n]$ the output is $$y[n] = h[n]*x[n]$$ In the frequency domain this
  is equivalent to
  $$Y\left(e^{j\omega}\right) = H\left(e^{j\omega}\right) \, X\left(e^{j\omega}\right)$$
  As in CT systems, convolution in the discrete-time domain is
  equivalent to multiplication in the frequency domain. Example: suppose
  a DT system has impulse response
  $$h[n] = \left( \gamma_1^n + \gamma_2^n \right)\, u[n]$$ and the input
  is $x[n] = n\, \gamma_3^n\, u[n]$ where $|\gamma_1| < 1$,
  $|\gamma_2| < 1$, $|\gamma_3| < 1$. The output in the frequency domain
  is
  \begin{aligned}
      Y\left(e^{j\omega}\right) &= H\left(e^{j\omega}\right) \, X\left(e^{j\omega}\right)\\
      &= \left[ \frac{1}{1-\gamma_1 e^{-j\omega}} + \frac{1}{1-\gamma_2 e^{-j\omega}} \right] \frac{\gamma_3 e^{-j\omega}}{\left( 1-\gamma_3 e^{-j\omega} \right)^2}\\
      &= \frac{\gamma_3 e^{-j\omega}}{\left(1-\gamma_1 e^{-j\omega}\right)\left( 1-\gamma_3 e^{-j\omega} \right)^2} + \frac{\gamma_3 e^{-j\omega}}{\left(1-\gamma_2 e^{-j\omega}\right)\left( 1-\gamma_3 e^{-j\omega} \right)^2} 
    
  \end{aligned}

- Multiplication (modulation) Property. Let
  $$x[n] \; \stackrel{\mathcal{F}}{\longleftrightarrow} \; X\left(e^{j\omega}\right)$$
  and
  $$y[n] \; \stackrel{\mathcal{F}}{\longleftrightarrow} \; Y\left(e^{j\omega}\right)$$
  then
  $$x[n]\,y[n] \; \stackrel{\mathcal{F}}{\longleftrightarrow} \; \frac{1}{2\pi} \int_{2\pi} X\left(e^{j\theta}\right)\, Y\left(e^{j(\omega-\theta)}\right)\; d\theta$$

## DT Fourier Transform of a Periodic Signal

The DTFS allows us to write any periodic function with period $N$ as
$$x[n] = \sum\limits_{k = N_0}^{N_0 + N -1} a_k e^{j\frac{2\pi}{N}kn}$$
taking the DT Fourier Transform
$$X\left(e^{j\omega}\right) = \sum\limits_{k = N_0}^{N_0 + N -1} a_k \mathcal{F}\left\{e^{j\frac{2\pi}{N}kn}\right\}$$
Using the previously derived transform shows, similar to CT, the DT
Fourier Transform of a periodic signal is
$$X\left(e^{j\omega}\right) = \sum\limits_{k = -\infty}^{\infty} 2\pi a_k \delta\left(\omega - \frac{2\pi k}{N}\right)$$

Example
$$x[n] = \cos\left(\frac{2\pi}{10} n\right) = \frac{1}{2}e^{j\frac{2\pi}{10} n} + \frac{1}{2}e^{-j\frac{2\pi}{10} n}$$
Using the previous transform
$$X\left(e^{j\omega}\right) =  \sum\limits_{k = -\infty}^{\infty} \pi \delta\left(\omega - \frac{2\pi}{10} -2\pi k\right) + \pi \delta\left(\omega + \frac{2\pi}{10} -2\pi k\right)$$
Which looks like

![Illustration of the Fourier spectrum of a DT periodic signal.](figures/fig17_5){fig-align="center" fig-alt="See the caption."}




